wired

Others/Aha.v
@@ -7,26 +7,26 @@ Inductive Term :=
 | t
 | f
 | zero
-| succ (t : Term)
-| pred (t : Term)
-| iszero (t : Term)
-| cond (p : Term) (t1 : Term) (t2 : Term).
+| succ      (t : Term)
+| pred      (t : Term)
+| iszero    (t : Term)
+| cond      (p : Term) (t1 : Term) (t2 : Term).
 
 Fixpoint isnv (t: Term) : bool :=
     match t with
-    | zero => true
-    | succ t' => isnv t'
-    | _ => false
+    | zero      => true
+    | succ t'   => isnv t'
+    | _         => false
     end.
 
 Fixpoint reduce (t : Term) : option Term :=
     match t with
     | cond t t1 _       => Some t1
-    | cond f _ t2       => Some t2
+    | cond f _  t2      => Some t2
     | cond k t1 t2      => option_map (fun z => cond z t1 t2) (reduce k)
     | succ n            => option_map succ (reduce n)
     | pred zero         => Some zero
-    | pred (succ n)     => if isnv n then Some f else None
+    | pred (succ n)     => if isnv n then Some n else None
     | pred n            => option_map pred (reduce n)
     | iszero zero       => Some t
     | iszero (succ n)   => if isnv n then Some f else None
@@ -47,7 +47,7 @@ Fixpoint depth (t : Term) : nat :=
 Lemma le_S : forall (a b : nat), a < b -> S a < S b. Proof. intros. lia. Qed.
 Lemma le_O : forall (a : nat), 0 < S a. Proof. intros. lia. Qed.
 
-(* the measufe might be wrong *)
+(* the measure might be wrong *)
 Function eval (t : Term) {measure depth t} : Term :=
     match reduce t with
     | None      => t
@@ -61,6 +61,64 @@ Proof.
         simpl. apply le_S.
         apply IHtm. reflexivity.
       + inversion H0.
-    - 
-      
+    - destruct (reduce tm) eqn: T.
+      + destruct tm; inversion T.
+        {
+            simpl in teq. destruct (isnv tm).
+            inversion H0. rewrite <- H2. simpl. 
+            lia. inversion H0.
+        }
+        {
+            simpl in H0. inversion H0. simpl.
+            assert (S (depth t0) < S(depth(pred tm))).
+            apply le_S. apply IHtm. reflexivity.
+            simpl in H. apply H.
+        }
+        {
+            simpl in H0. inversion H0. 
+            assert (S (depth t0) < S(depth(iszero tm))).
+            apply le_S. apply IHtm. reflexivity.
+            simpl in H. apply H.
+        }
+        {
+            simpl in H0. inversion H0.
+            assert (S (depth t0) < S(depth(cond tm1 tm2 tm3))).
+            apply le_S. apply IHtm. reflexivity.
+            simpl in H. apply H.
+        } 
+     + destruct tm; inversion H0.
+       { auto. }
+       { 
+            destruct (isnv tm); inversion H1.
+            simpl. lia.
+       }
+    - destruct (reduce tm) eqn: T.
+      + destruct tm; inversion T.
+        {
+            simpl in teq. destruct (isnv tm); inversion H0.
+            simpl. lia.
+        }
+        {
+            simpl in teq. destruct (isnv tm);
+            simpl in H0; inversion H0;
+            assert (S (depth t0) < S(depth (pred tm)));
+            simpl; apply le_S; apply IHtm; reflexivity;
+            apply H.
+        }
+        {
+            simpl in H0. inversion H0.
+            assert (S (depth t0) < S (depth (iszero tm))).
+            apply le_S. apply IHtm. reflexivity. apply H.
+        }
+        {
+            simpl in H0. inversion H0.
+            assert (S (depth t0) < S(depth(cond tm1 tm2 tm3))).
+            apply le_S. apply IHtm. reflexivity.
+            simpl in H. apply H.
+        }
+      + destruct tm; inversion H0.
+        
+
 Abort.
+
+Compute (reduce (iszero zero)).
